get_exists_matching_src_ips_executable

Bitmagic/WordInterval_Lists.thy
@@ -74,4 +74,19 @@ text{*A list of @{text "(start, end)"} tuples.*}
   lemma l2br_negation_type_intersect: "wordinterval_to_set (l2br_negation_type_intersect l) = 
                         (\<Inter> (i,j) \<in> set (getPos l). {i .. j}) - (\<Union> (i,j) \<in> set (getNeg l). {i .. j})"
     by(simp add: l2br_negation_type_intersect_alt l2br_intersect l2br)
+
+
+  fun l2br_negation_type_union :: "('a::len word \<times> 'a::len word) negation_type list \<Rightarrow> 'a::len wordinterval" where
+    "l2br_negation_type_union [] = Empty_WordInterval" |
+    "l2br_negation_type_union ((Pos (s,e))#ls) = wordinterval_union (WordInterval s e) (l2br_negation_type_union ls)" |
+    "l2br_negation_type_union ((Neg (s,e))#ls) = wordinterval_union (wordinterval_invert (WordInterval s e)) (l2br_negation_type_union ls)"
+
+
+  lemma l2br_negation_type_union: "wordinterval_to_set (l2br_negation_type_union l) = 
+                        (\<Union> (i,j) \<in> set (getPos l). {i .. j}) \<union> (\<Union> (i,j) \<in> set (getNeg l). - {i .. j})"
+  apply(simp add: l2br)
+  apply(induction l rule: l2br_negation_type_union.induct)
+    apply(simp_all)
+   apply fast+
+  done
 end
